proof/crefine/RISCV64/Detype_C.thy
@@ -397,6 +397,32 @@ proof -
   qed
 qed
 
+lemma ko_at_is_aligned' [intro?]:
+  "ko_at' ko p s \<Longrightarrow> is_aligned p (objBits ko)"
+  apply (erule obj_atE')
+  apply (simp add: objBits_def project_inject)
+  done
+
+(* FIXME RT: write valid_untyped_cap_ko_at_disjoint with intvl notation? *)
+lemma valid_untyped_cap_ko_at_disjoint':
+  assumes vu: "s \<turnstile>' UntypedCap d ptr bits idx"
+  and   koat: "ko_at' ko x s"
+  and     pv: "{x..+2 ^ objBits ko} \<inter> {ptr..+2 ^ bits} \<noteq> {}"
+  shows   "{x..+2 ^ objBits ko} \<subseteq> {ptr..+2 ^ bits}"
+  apply (insert assms)
+  apply (frule (1) valid_untyped_cap_ko_at_disjoint)
+   apply (subst upto_intvl_eq[symmetric])
+    apply (erule ko_at_is_aligned')
+   apply (subst upto_intvl_eq[symmetric])
+    apply (clarsimp simp: valid_cap'_def capAligned_def)
+   apply fastforce
+  apply (subst upto_intvl_eq)
+   apply (erule ko_at_is_aligned')
+  apply (subst upto_intvl_eq)
+   apply (clarsimp simp: valid_cap'_def capAligned_def)
+  apply simp
+  done
+
 (* FIXME x64: tcb bits change *)
 lemma tcb_ptr_to_ctcb_ptr_in_range:
   fixes tcb :: tcb
@@ -482,12 +508,6 @@ proof -
       done
   qed
 qed
-
-lemma ko_at_is_aligned' [intro?]:
-  "ko_at' ko p s \<Longrightarrow> is_aligned p (objBits ko)"
-  apply (erule obj_atE')
-  apply (simp add: objBits_def project_inject)
-  done
 
 lemma cmap_relation_disjoint_tcb:
   fixes x :: "tcb_C ptr"
@@ -858,6 +878,187 @@ proof -
       done
   qed
 qed
+
+lemma sched_context_disjoint:
+  fixes x :: "sched_context_C ptr"
+  assumes vuc: "s \<turnstile>' UntypedCap d ptr bits idx"
+  and    invs: "invs' s"
+  and      cm: "cmap_relation (projectKO_opt \<circ>\<^sub>m (ksPSpace s)) (cslift s') Ptr csched_context_relation"
+  and      xv: "x \<notin> Ptr ` {ptr..+2 ^ bits}"
+  and      sc: "ko_at' (sc :: sched_context) (ptr_val x) s"
+  shows  "{ptr_val x..+2 ^ objBits  sc} \<inter> {ptr..+2 ^ bits} = {}"
+proof -
+  from vuc have al: "is_aligned ptr bits" and vu: "valid_untyped' d ptr bits idx s" and p0: "ptr \<noteq> 0"
+    and wb: "bits < word_bits" and [simp]: "(ptr && ~~ mask bits) = ptr"
+    by (auto elim!: valid_untyped_capE)
+
+  note [simp del] = atLeastAtMost_simps
+
+  let ?ran = "{ptr..ptr + 2 ^ bits - 1}"
+  let ?s = "(s\<lparr>ksPSpace := (ksPSpace s) |` (- ?ran)\<rparr>)"
+
+  let ?oran = "{ptr_val x .. ptr_val x + 2 ^ objBitsKO (KOSchedContext sc) - 1}"
+
+  let ?ran' = "{ptr..+2 ^ bits}"
+  let ?oran' = "{ptr_val x..+2 ^ objBitsKO (KOSchedContext sc)}"
+
+  have ran' [simp]: "?ran' = ?ran" using al wb upto_intvl_eq by auto
+
+  have oran' [simp]: "?oran' = ?oran"
+  proof (rule upto_intvl_eq)
+    show "is_aligned (ptr_val x) (objBitsKO (KOSchedContext sc))"
+      using sc invs by (fastforce simp: obj_at_simps intro: pspace_alignedD')
+  qed
+
+  from xv have px: "ptr_val x \<in> (- ?ran)"
+    apply (simp only: ran' Compl_iff)
+    apply (erule contrapos_nn)
+    apply (erule image_eqI [rotated])
+    apply simp
+    done
+
+  hence "ksPSpace ?s (ptr_val x) = Some (KOSchedContext sc)" using sc by (simp add: obj_at_simps)
+  hence "?oran \<inter> ?ran = {}"
+  proof (rule pspace_no_overlapD'[where p = ptr and bits = bits,simplified])
+    from invs have "valid_pspace' s" ..
+    with vu al show "pspace_no_overlap' ptr bits ?s" using valid_untyped_no_overlap
+        by (clarsimp simp: mask_def add_diff_eq)
+  qed
+
+  hence "?oran' \<inter> ?ran' = {}" by simp
+  thus "{ptr_val x..+2 ^ objBits sc} \<inter> ?ran' = {}"
+  proof (rule disjoint_subset [rotated])
+    show "{ptr_val x..+2 ^ objBits sc} \<subseteq> ?oran'"
+      apply -
+      apply (rule intvl_start_le)
+      apply (simp add: size_of_def objBits_simps)
+      done
+  qed
+qed
+
+lemma minSchedContextBits_check:
+  "minSchedContextBits =
+   (LEAST n. size_of TYPE(sched_context_C) + MIN_REFILLS * size_of TYPE(refill_C) \<le> 2 ^ n)"
+sorry
+
+lemma schedContextStructSize_minSchedContextBits:
+  "size_of TYPE(sched_context_C) \<le> 2 ^ minSchedContextBits"
+  apply (insert minSchedContextBits_check)
+  by (metis LeastI_ex add_leD1 le_refl self_le_ge2_pow)
+
+lemma schedContextStructSize_sizeof:
+  "schedContextStructSize = size_of TYPE(sched_context_C)"
+  by (simp add: sc_const_eq sizeof_sched_context_t_def word_size_def)
+
+lemma refillSizeBytes_sizeof:
+  "refillSizeBytes = size_of TYPE(refill_C)"
+  by (simp add: refillSizeBytes_def)
+
+lemma refillAbsoluteMax'_leq:
+  "size_of TYPE(sched_context_C) \<le> 2 ^ n \<Longrightarrow>
+   size_of TYPE(sched_context_C) + (refillAbsoluteMax' n) * size_of TYPE(refill_C) \<le> 2 ^ n"
+  supply refill_C_size[simp del] sched_context_C_size[simp del]
+  apply (simp add: max_num_refills_eq_refillAbsoluteMax'[symmetric] max_num_refills_def
+                   scBits_simps(4) scBits_simps(3)
+                   schedContextStructSize_sizeof refillSizeBytes_sizeof)
+  by (metis Nat.le_diff_conv2 Nat.le_imp_diff_is_add div_times_less_eq_dividend nat_iffs(1)
+            nat_simps(2))
+
+lemma scRefills_sc_size_rel:
+  "valid_sched_context' sc s \<Longrightarrow>
+   size_of TYPE(sched_context_C) +  length (scRefills sc) * size_of TYPE(refill_C)
+   \<le> 2 ^ objBitsKO (KOSchedContext sc)"
+  supply refill_C_size[simp del] sched_context_C_size[simp del]
+  apply (clarsimp simp: objBits_simps valid_sched_context'_def add_ac)
+  apply (rule refillAbsoluteMax'_leq)
+  apply (rule_tac y="2 ^ minSchedContextBits" in order_trans)
+   apply (rule schedContextStructSize_minSchedContextBits)
+  by fastforce
+
+lemma refillSizeBytes_nonzero:
+  "0 < refillSizeBytes"
+  by (simp add: refillSizeBytes_def)
+
+lemma refill_intvl_self:
+  "ptr_val (PTR(refill_C) x) \<in> {x..+size_of TYPE(refill_C)}"
+  by (fastforce intro: intvl_self)
+
+lemma refill_within_sc_size:
+  "\<lbrakk>ko_at' sc p s; valid_sched_context' sc s; pspace_bounded' s;
+    sc_ptr_to_crefill_ptr p +\<^sub>p int n = PTR(refill_C) x; n < length (scRefills sc) \<rbrakk>
+   \<Longrightarrow> {x..+size_of TYPE(refill_C)} \<subseteq> {p..+2 ^ objBits sc}"
+  supply refill_C_size[simp del] sched_context_C_size[simp del]
+  apply (insert scRefills_sc_size_rel[where sc=sc and s=s])
+  apply (simp add: sc_ptr_to_crefill_ptr_def schedContextStructSize_sizeof refillSizeBytes_sizeof)
+  apply (drule sym)
+  apply clarsimp
+  apply (subgoal_tac "{p + word_of_nat (size_of TYPE(sched_context_C)) +
+                       word_of_nat n * word_of_nat (size_of TYPE(refill_C))..+size_of TYPE(refill_C)}
+                      \<subseteq> {p..+2 ^ objBits sc}")
+   apply fastforce
+  apply (prop_tac "{p + word_of_nat (size_of TYPE(sched_context_C)) +
+                    word_of_nat n * word_of_nat (size_of TYPE(refill_C))..+size_of TYPE(refill_C)}
+                   = {p + word_of_nat (size_of TYPE(sched_context_C) +
+                      n * size_of TYPE(refill_C))..+size_of TYPE(refill_C)} ")
+   apply (simp add: word_of_nat_plus add_ac)
+  apply (simp only:)
+  apply (rule intvl_sub_offset)
+  apply (frule pspace_boundedD'[rotated])
+   apply (fastforce simp: obj_at_simps)
+  apply (subst unat_of_nat_eq)
+   apply (rule_tac y="2 ^ objBits sc" in le_less_trans)
+    using word_bits_def
+    by (fastforce simp: refill_C_size objBits_simps)+
+
+lemma sc_from_refill:
+  "\<lbrakk>clift (t_hrs_' (globals s')) (x :: refill_C ptr) = Some refill;
+    refill_buffer_relation (ksPSpace s) (t_hrs_' (globals s')) (ghost'state_' (globals s'));
+    invs' s\<rbrakk>
+   \<Longrightarrow> \<exists>p sc n. ko_at' sc p s
+                \<and> {ptr_val x..+size_of TYPE(refill_C)} \<subseteq> {p..+2 ^ objBits sc}
+                \<and> ptr_val x \<in> {p..+2 ^ objBits sc}
+                \<and> n < length (scRefills sc)
+                \<and> x = sc_ptr_to_crefill_ptr p +\<^sub>p int n"
+  supply refill_C_size[simp del]
+  apply (frule refill_buffer_relation_crefill_hp_dom)
+  apply (clarsimp simp: Let_def)
+  apply (drule equalityD1)
+  apply (prop_tac "x \<in> dom (clift (t_hrs_' (globals s')))")
+   apply fastforce
+  apply (drule (1) set_rev_mp)
+  apply clarsimp
+  apply (rename_tac p n sc)
+  apply (rule_tac x=p in exI)
+  apply (rule_tac x=sc in exI)
+  apply (intro context_conjI; fastforce?)
+   apply (fastforce intro: map_to_ko_atI')
+  by (frule_tac x="ptr_val x" in refill_within_sc_size;
+      fastforce dest: sc_ko_at_valid_objs_valid_sc')
+
+lemma refill_disjoint:
+  fixes x :: "refill_C ptr"
+  assumes vuc: "s \<turnstile>' UntypedCap d ptr bits idx"
+  and    invs: "invs' s"
+  and      ht: "s' \<Turnstile>\<^sub>c x"
+  and     rel: "refill_buffer_relation (ksPSpace s) (t_hrs_' (globals s')) (ghost'state_' (globals s'))"
+  and      cm: "cmap_relation (projectKO_opt \<circ>\<^sub>m (ksPSpace s)) (cslift s') Ptr csched_context_relation"
+  and      xv: "x \<notin> Ptr ` {ptr..+2 ^ bits}"
+  shows  "{ptr_val x..+size_of TYPE(refill_C)} \<inter> {ptr..+2 ^ bits} = {}"
+  apply (insert assms)
+  apply (prop_tac "\<exists>refill. cslift s' x = Some refill")
+   apply (clarsimp simp: clift_Some_eq_valid)
+  apply clarsimp
+  apply (frule_tac x=x in sc_from_refill[rotated])
+    apply clarsimp
+   apply fastforce
+  apply clarsimp
+  apply (rename_tac p sc n)
+  apply (frule_tac x="Ptr p" and sc=sc in sched_context_disjoint; fastforce?)
+  apply clarsimp
+  apply (frule (1) valid_untyped_cap_ko_at_disjoint')
+   apply (fastforce intro!: intvl_self)
+  apply force
+  done
 
 lemma tcb_queue_relation_live_restrict':
   assumes vuc: "s \<turnstile>' capability.UntypedCap d ptr bits idx"
@@ -1502,6 +1703,10 @@ lemma zero_ranges_are_zero_typ_region_bytes:
   apply (clarsimp simp: region_actually_is_bytes'_def typ_region_bytes_def hrs_htd_update)
   done
 
+lemma rev_bexI':
+  "x \<in> A \<and> P x \<Longrightarrow> \<exists>x\<in>A. P x"
+  by fastforce
+
 lemma deleteObjects_ccorres':
   notes if_cong[cong]
   shows
@@ -1643,14 +1848,17 @@ proof -
     using cendpoint_relation_restrict [OF D.valid_untyped invs sym_refs rl]
       cnotification_relation_restrict [OF D.valid_untyped invs sym_refs rl]
     using  cmap_array[simplified bit_simps]
+    supply sched_context_C_size[simp del] sched_context_C_size_of[simp del]
     apply -
     apply (elim conjE)
     apply ((subst lift_t_typ_region_bytes,
            rule cm_disj cm_disj_tcb cm_disj_cte cm_disj_user cm_disj_device, assumption+,
-           simp_all add: objBits_simps' bit_simps scBits_simps
-                         heap_to_user_data_restrict heap_to_device_data_restrict)[1],
-           (rule_tac y="2^7" in order_trans, simp,
-            fastforce intro!: power_increasing_iff[THEN iffD2] scBits_at_least_7)?)+
+           simp_all add: objBits_simps' bit_simps
+                         heap_to_user_data_restrict heap_to_device_data_restrict
+                         schedContextStructSize_sizeof[unfolded size_of_def, symmetric]
+                         schedContextStructSize_sizeof)[1],
+           (rule_tac y="2 ^ minSchedContextBits" in order_trans,
+            rule schedContextStructSize_minSchedContextBits, fastforce)?)+
     apply (simp add: map_to_ctes_delete' cmap_relation_restrict_both_proj
                      cmap_relation_restrict_both cmap_array_helper hrs_htd_update
                      bit_simps cmap_array)
@@ -1921,12 +2129,63 @@ proof -
     apply (simp add: cinterrupt_relation_def cte_level_bits_def)
     done
 
-  (* FIXME RT *)
   moreover from sr have
-    "refill_buffer_relation (ksPSpace s|\<^bsub>(- intvl (ptr, 2 ^ bits))\<^esub>)
-                              (hrs_htd_update (typ_region_bytes ptr bits) (t_hrs_' (globals s')))
+    "refill_buffer_relation (ksPSpace s|`(- {ptr..+2 ^ bits}))
+                            (hrs_htd_update (typ_region_bytes ptr bits) (t_hrs_' (globals s')))
                             (gs_clear_region ptr bits (ghost'state_' (globals s')))"
-    sorry
+    apply (insert sr invs)
+    apply (frule rf_sr_refill_buffer_relation)
+    apply (simp only: refill_buffer_relation_def Let_def)
+    apply (subst lift_t_typ_region_bytes)
+      subgoal by (fastforce dest!: refill_disjoint[OF D.valid_untyped invs])
+     apply fastforce
+    apply (subst lift_t_typ_region_bytes)
+      subgoal by (fastforce dest!: refill_disjoint[OF D.valid_untyped invs])
+     apply fastforce
+    apply (intro context_conjI)
+       apply (frule rf_sr_refill_buffer_relation)
+       apply (simp only: set_eq_subset)
+       apply (rule conjI)
+        apply clarsimp
+        apply (frule (2) sc_from_refill)
+        apply clarsimp
+        apply (rename_tac p sc n)
+        apply (rule_tac x=p in rev_bexI')
+        apply (rule context_conjI)
+         apply (simp add: map_comp_restrict_map)
+         apply (rule conjI)
+          apply (force simp: obj_at_simps)
+         apply clarsimp
+         apply (frule valid_untyped_cap_ko_at_disjoint'[OF D.valid_untyped])
+          subgoal by (fastforce intro!: intvl_self)
+         apply (force simp: image_def)
+        apply (force simp: obj_at_simps map_comp_def restrict_map_def split: if_splits)
+       apply clarsimp
+       apply (rule conjI)
+        apply (fastforce simp: map_comp_def restrict_map_def split: if_splits)
+       apply clarsimp
+       apply (rename_tac p n refill sc)
+       apply (prop_tac "ko_at' sc p s")
+        apply (fastforce intro: map_to_ko_atI'
+                          simp: map_comp_def restrict_map_def
+                         split: if_splits)
+       apply (frule_tac x="PTR(sched_context_C) p" in sched_context_disjoint[OF D.valid_untyped])
+          apply fastforce
+         apply clarsimp
+        apply fastforce
+       apply (frule (1) invs'_ko_at_valid_sched_context')
+       apply (insert refill_intvl_self)
+       apply (fastforce dest!: refill_within_sc_size)
+      apply (clarsimp simp: dyn_array_list_rel_pointwise)
+      apply (elim allE)
+      apply (clarsimp simp: map_comp_def restrict_map_def split: if_splits)
+      apply (prop_tac "sc_ptr_to_crefill_ptr p +\<^sub>p int n
+                       \<in> dom (cslift s'|`(- PTR(refill_C) ` {ptr..+2 ^ bits}))")
+       apply clarsimp
+       apply (force intro!: bexI)
+      apply (force simp: restrict_map_def)
+     subgoal by (auto simp: gs_clear_region_def dom_def map_comp_def restrict_map_def)
+    by (auto simp: gs_clear_region_def map_comp_def)
 
   ultimately
   show "(?t, globals_update
