proof/crefine/RISCV64/SR_lemmas_C.thy
@@ -2106,6 +2106,11 @@ lemma rf_sr_sched_action_relation:
    \<Longrightarrow> cscheduler_action_relation (ksSchedulerAction s) (ksSchedulerAction_' (globals s'))"
   by (clarsimp simp: rf_sr_def cstate_relation_def Let_def)
 
+lemma rf_sr_refill_buffer_relation[intro]:
+  "(s, s') \<in> rf_sr \<Longrightarrow>
+   refill_buffer_relation (ksPSpace s) (t_hrs_' (globals s')) (ghost'state_' (globals s'))"
+  by (clarsimp simp: rf_sr_def cstate_relation_def Let_def)
+
 lemma canonical_address_tcb_ptr:
   "\<lbrakk>canonical_address t; is_aligned t tcbBlockSizeBits\<rbrakk> \<Longrightarrow>
      canonical_address (ptr_val (tcb_ptr_to_ctcb_ptr t))"
